Foundation/Propositional/Kripke2/AxiomD.lean
@@ -18,34 +18,24 @@ namespace Frame
 protected abbrev IsSerial (F : Kripke2.Frame) := _root_.IsSerial F.Rel
 lemma serial [F.IsSerial] : ∀ x : F, ∃ y, x ≺ y := IsSerial.serial
 
-protected class IsWeakSerial (F : Kripke2.Frame) where
-  weak_serial : ∀ {x y : F}, x ≺ y → ∃ z, y ≺ z
-export IsWeakSerial (weak_serial)
-
-instance [F.IsSerial] : F.IsWeakSerial := ⟨by
-  intro _ y _;
-  obtain ⟨z, Ryz⟩ := F.serial y;
-  use z;
-⟩
-
 end Frame
 
 
 @[simp high, grind .]
-lemma valid_axiomD_of_isWeakSerial [F.IsWeakSerial] : F ⊧ ∼∼⊤ := by
+lemma valid_axiomD_of_isSerial [F.IsSerial] : F ⊧ ∼∼⊤ := by
   intro V x y Rxy h;
   contrapose! h;
   apply Satisfies.not_def_neg.mpr;
-  obtain ⟨z, Ryz⟩ := F.weak_serial Rxy;
+  obtain ⟨z, Ryz⟩ := F.serial y;
   use z;
   constructor;
   . assumption;
   . exact Satisfies.def_top
 
-lemma isWeakSerial_of_valid_axiomD (h : F ⊧ ∼∼⊤) : F.IsWeakSerial := by
+lemma isSerial_of_valid_axiomD (h : F ⊧ ∼∼⊤) : F.IsSerial := by
   constructor;
   intro x;
-  simpa [Satisfies] using @h (λ v a => True) x;
+  simpa [Satisfies] using @h (λ v a => True) F.root x F.rooted;
 
 end Kripke2
 
