Foundation/Propositional/Kripke2/AxiomRfl.lean
@@ -1,0 +1,45 @@
+import Foundation.Propositional.Kripke2.Basic
+import Foundation.Vorspiel.HRel.Convergent
+import Foundation.Vorspiel.HRel.Euclidean
+import Foundation.Vorspiel.HRel.Coreflexive
+
+namespace LO.Propositional
+
+open Kripke2
+open Formula.Kripke2
+
+namespace Kripke2
+
+variable {F : Kripke2.Frame}
+
+
+namespace Frame
+
+protected abbrev IsReflexive (F : Kripke2.Frame) := _root_.IsRefl _ F.Rel
+@[simp, grind .] lemma refl [F.IsReflexive] : ∀ x : F, x ≺ x := IsRefl.refl
+
+end Frame
+
+
+@[simp high, grind .]
+lemma valid_axiomRfl_of_isReflexive [F.IsReflexive] : F ⊧ (φ ⋏ (φ ➝ ψ)) ➝ ψ := by
+  intro V x y Rxy h;
+  have ⟨h₁, h₂⟩ := Satisfies.def_and.mp h;
+  apply h₂;
+  . simp;
+  . assumption;
+
+lemma isReflexive_of_valid_axiomRfl (h : F ⊧ ((.atom 0) ⋏ ((.atom 0) ➝ (.atom 1))) ➝ (.atom 1)) : F.IsReflexive := by
+  constructor;
+  intro x;
+  have := @h (λ w a => match a with | 0 => w = x | 1 => x ≺ w | _ => False) F.root x F.rooted $ by
+    apply Satisfies.def_and.mpr;
+    constructor;
+    . tauto;
+    . rintro y Rxy;
+      tauto;
+  exact this;
+
+end Kripke2
+
+end LO.Propositional
